src/Phasers/Phasermap.v
@@ -130,6 +130,14 @@ Inductive In (t:tid) (pm:phasermap) : Prop :=
     Map_TID.In t ph ->
     In t pm.
 
+Inductive Nonempty (pm:phasermap) : Prop :=
+| nonempty_def:
+  forall x,
+  In x pm ->
+  Nonempty pm.
+
+Definition Empty (pm:phasermap) : Prop := forall x, ~ In x pm.
+
 (** The parameter of a phased async is list of pairs, each of which
   consists of a phaser name and a registration  mode. *)
 
@@ -211,10 +219,10 @@ Inductive Reduces m t o : phasermap -> Prop :=
     can_run (get_impl o) t m ->
     Reduces m t o (run (get_impl o) t m).
 
-Section Defs.
-  Definition trace := (list (tid * op)) % type.
+Module Trace.
+  Definition t := (list (tid * op)) % type.
 
-  Inductive ReducesN: phasermap -> trace -> Prop :=
+  Inductive ReducesN: phasermap -> t -> Prop :=
   | reduces_n_nil:
     ReducesN make nil
   | reduces_n_cons:
@@ -222,21 +230,7 @@ Section Defs.
     ReducesN pm l ->
     Reduces pm t o pm' ->
     ReducesN pm' ((t,o)::l).
-
-  Structure phasermap_t := {
-    state : phasermap;
-    history : trace;
-    phasermap_spec: ReducesN state history
-  }.
-
-  Inductive ReducesT: phasermap_t -> (tid*op) -> phasermap_t -> Prop :=
-  | reduces_t_def:
-    forall t o pm1 pm2,
-    Reduces (state pm1) t o (state pm2) ->
-    history pm2 = (t,o)::(history pm1) ->
-    ReducesT pm1 (t, o) pm2.
-
-End Defs.
+End Trace.
 
 Section Facts.
 
