src/Finish/DF.v
@@ -1,0 +1,125 @@
+Require Import Vars.
+Require Import Syntax2.
+Require Import Coq.Lists.List.
+Import ListNotations.
+
+Section Defs.
+  Structure t := make {
+    state : state;
+    history : Trace.t;
+    spec: Trace.ReducesN state history
+  }.
+
+  (** A typed reduction *)
+
+  Inductive Reduces: t -> (tid*op) -> t -> Prop :=
+  | reduces_def:
+    forall t o pm1 pm2,
+    Syntax2.Reduces (state pm1) (t, o) (state pm2) ->
+    history pm2 = (t,o)::(history pm1) ->
+    Reduces pm1 (t, o) pm2.
+End Defs.
+
+Section Props.
+(*
+  Let progress_aux:
+    forall o x m s',
+    Syntax2.Reduces (state m) (x, o) s' ->
+    exists n, Reduces m (x, o) n.
+  Proof.
+    intros.
+    eapply Trace.reduces_n_cons; eauto.
+  Qed.
+*)
+
+  Program Definition reduces_step_aux
+    x o (s:t) s'
+    (Hr: Syntax2.Reduces (state s) (x, o) s') :=
+    {| state := s'; history := (x,o)::(history s) |}.
+  Next Obligation.
+    destruct s.
+    eapply Trace.reduces_n_cons; eauto.
+  Qed. (* leave it open *)
+
+  Lemma reduces_step:
+    forall x o s s' (X : Syntax2.Reduces (state s) (x, o) s'),
+    exists s',
+    Reduces s (x, o) s'.
+  Proof.
+    intros.
+    exists (reduces_step_aux x o s s' X).
+    eauto using reduces_def.
+  Qed.
+
+  (** An enabled task can reduce with any operation. *)
+  Definition Enabled s t :=
+  forall o, Valid (state s) t o -> exists s', Reduces s (t, o) s'.
+
+  Let enabled_to_enabled:
+    forall s t,
+    Syntax2.Enabled (state s) t ->
+    Enabled s t.
+  Proof.
+    intros.
+    unfold Enabled, Syntax2.Enabled in *.
+    intros ? Hv.
+    apply H in Hv.
+    destruct Hv as (s', Hr).
+    eauto using reduces_step.
+  Qed.
+
+  Corollary progress_ex:
+    forall (s:t),
+    (* And that state is not empty *)
+    ~ Map_TID.Empty (state s) ->
+    (* Then there is some [f] such that *)
+    exists f,
+    ((* [f] is nonempty and every task in [f] reduces. *)
+      Nonempty f (state s)
+      /\
+      forall t, Root t f (state s) -> Enabled s t
+    )
+    \/
+    ((* Or [f] is empty, and [t]'s current finish-scope is [f] *)
+      Empty f (state s)
+      /\
+      exists t, Current t f (state s) /\ Enabled s t
+    ).
+  Proof.
+    intros.
+    edestruct Trace.progress_ex as (f,[(Hx,Hy)|(Hx,(x,(Hy,Hz)))]); eauto using spec;
+    exists f. {
+      left.
+      split; auto.
+    }
+    right.
+    split; auto.
+    exists x.
+    split; auto.
+  Qed.
+
+  Lemma progress_nonblocking:
+    forall s t o,
+    Valid (state s) t o ->
+    o <> AWAIT ->
+    exists s', Reduces s (t, o) s'.
+  Proof.
+    intros.
+    eapply progress_nonblocking in H; eauto using spec.
+    destruct H as (s', H).
+    eauto using reduces_step.
+  Qed.
+
+  Theorem progress:
+    forall s,
+    ~ Map_TID.Empty (state s) ->
+    (* Then there is some [f] such that *)
+    exists t,
+    Enabled s t.
+  Proof.
+    intros.
+    eapply Trace.progress in H; eauto using spec.
+    destruct H as (t, Hx);
+    eauto using enabled_to_enabled.
+  Qed.
+End Props.
