src/Phasers/DF.v
@@ -1,0 +1,97 @@
+Require Import Coq.Lists.List.
+Import ListNotations.
+
+Require Import Lang.
+Require Import Vars.
+Require HJ.Phasers.Typesystem.
+Require HJ.Phasers.WellFormed.
+Require HJ.Phasers.Progress.
+Require HJ.Phasers.SubjectReduction.
+Require Import HJ.Phasers.Phasermap.
+Section Defs.
+
+  Structure t := {
+    state : phasermap;
+    history : Trace.t;
+    spec: Trace.ReducesN state history
+  }.
+
+  Inductive Reduces: t -> (tid*op) -> t -> Prop :=
+  | reduces_def:
+    forall t o pm1 pm2,
+    Phasermap.Reduces (state pm1) t o (state pm2) ->
+    history pm2 = (t,o)::(history pm1) ->
+    Reduces pm1 (t, o) pm2.
+
+  Lemma make : t.
+  Proof.
+    refine ({| state := make; history := nil |}).
+    auto using Trace.reduces_n_nil.
+  Qed.
+
+End Defs.
+
+Section Props.
+  Let progress_aux:
+    forall o x m s',
+    Phasermap.Reduces (state m) x o s' ->
+    exists n, Reduces m (x, o) n.
+  Proof.
+    intros.
+    assert (Hr: Trace.ReducesN s' ( (x,o)::(history m))%list ). {
+      eauto using Trace.reduces_n_cons, spec.
+    }
+    exists {|
+      state := s';
+      history := ((x,o)::(history m))%list;
+      spec := Hr
+    |}.
+    eauto using reduces_def.
+  Qed.
+
+  Definition Enabled s x :=
+  forall o,
+  Typesystem.Op.Valid (state s) x o -> exists q, Reduces s (x, o) q.
+
+  Theorem progress:
+    forall (s:t),
+    Nonempty (state s) ->
+    exists x, In x (state s) /\ Enabled s x.
+  Proof.
+    intros.
+    apply Progress.progress in H;
+    eauto using
+      SubjectReduction.reduces_n_to_valid,
+      spec,
+      WellFormed.Phasermap.well_formed_to_reduces_n.
+    destruct H as (x, (Hi, He)).
+    exists x.
+    unfold Enabled; split; auto.
+    intros.
+    edestruct He; eauto.
+  Qed.
+  
+  Theorem progress_empty:
+    forall (s:t),
+    Empty (state s) ->
+    forall x, Enabled s x.
+  Proof.
+    intros.
+    apply LEDec.pm_tids_empty in H.
+    unfold Enabled; intros.
+    edestruct Progress.progress_empty; eauto using spec.
+  Qed.
+
+  Lemma progress_unblocking:
+    forall pm t i,
+    i <> WAIT_ALL ->
+    Typesystem.Op.Valid (state pm) t i ->
+    exists m, Reduces pm (t, i) m.
+  Proof.
+    intros.
+    eapply Progress.progress_unblocking_simple in H; eauto using spec, SubjectReduction.reduces_n_to_valid.
+    destruct H as (m', Hr).
+    eauto.
+  Qed.
+
+End Props.
